vehicle1_bad.pml
@@ -1,0 +1,127 @@
+/* Simple 3 vehicle example with leader (who just sends),
+ * vehicle, who receives from both leader and tail, and
+ * tail, who just sends:  leader --> vehicle <-- tail */
+
+/* Round robin:
+   (clock%3)=0 -> leader; (clock%3)=1 -> vehicle; (clock%3)=2 -> tail */
+
+int clock; 
+int lspeed = 0;
+int vspeed = 0;
+int tspeed = 0;
+
+proctype leader(int vnum; chan out)  /* leader vehicle */
+{
+   printf("leader: starting\n"); 
+
+   L1: (clock%3) == vnum; /* wait for my turn */
+       printf("leader: my turn\n");
+       if
+	  :: (clock > 100) -> goto FIN
+       	  :: (clock <= 100) ->
+	     	    out!(clock%5);
+		    lspeed=(clock%5);
+	     	    printf("leader: speed %d\n", (clock%5));		    
+    		    clock++;
+		    goto L1
+	fi;
+	FIN: clock++; printf("leader: finishing\n")
+}
+
+proctype vehicle(int vnum; chan l_in, t_in)   /* vehicle */
+{
+   printf("vehicle: starting\n"); 
+   int lin1, tin1;
+
+   V1: (clock%3) == vnum; /* wait for my turn */
+       printf("vehicle: my turn\n");
+       /* if we receive no speeds, keep the same value;
+          if we receive one speed, set our speed to that;
+	  if we receive two speed messages, set our speed to average (rounded down)
+	*/
+       if
+	  :: (clock > 100) -> goto FIN;
+       	  :: (clock <= 100) ->
+      	     	    if
+	     	    :: ((len(l_in)==0) && (len(t_in)==0))
+		       ->  printf("vehicle: no msgs\n")
+	     	    :: ((len(l_in)!=0) && (len(t_in)==0)) 
+		       ->  l_in?lin1; printf("vehicle: received and adjust speed (%d)\n", lin1); lspeed=lin1
+	     	    :: ((len(l_in)==0) && (len(t_in)!=0))
+		       ->  t_in?tin1; printf("vehicle: received and adjust speed (%d)\n", tin1); lspeed=tin1
+	      	    :: ((len(l_in)!=0) && (len(t_in)!=0))
+		       ->  l_in?lin1; t_in?tin1; vspeed = (lin1 + tin1)/2;
+		           printf("vehicle: received (%d,%d) and adjusted speed to %d\n", lin1, tin1, vspeed)
+                    fi;
+       		    clock++; 
+		    goto V1   		   
+        fi;
+   	FIN: /* vspeed = 300; */ clock++; printf("vehicle: finishing\n")
+}
+
+proctype tail(int vnum; chan out)  /* tail vehicle */
+{
+   printf("tail: starting\n"); 
+
+   T1: (clock%3) == vnum; /* wait for my turn */
+       printf("tail: my turn\n");
+       if
+	  :: (clock > 100) -> goto FIN;
+       	  :: (clock <= 100) ->
+	     	    out!(clock%5);
+		    tspeed=(clock%5);
+	     	    printf("tail: speed %d\n", (clock%5));		    
+    		    clock++;
+		    goto T1
+	fi;
+	FIN: clock++; printf("tail: finishing\n")
+}
+
+proctype attacker(chan l_in, t_in)   /* attackder */
+{
+   printf("attacker: starting\n"); 
+   int lin1, tin1;
+
+   (clock > 10); /* wait until under way */
+   
+   if
+	:: (clock%55) == 0 -> printf("attacker: inserting vspeed of 100\n"); l_in!100; l_in!100
+	:: (clock%66) == 0 -> printf("attacker: inserting tspeed of 123\n"); t_in!123; t_in!123
+	:: (clock>100) -> goto FIN;
+   fi;
+   FIN:  printf("attacker: finishing\n")
+}
+
+init
+{
+  clock = 0; printf("Starting 0\n");
+  chan v1tov2 = [10] of { int };
+  chan v3tov2 = [10] of { int };
+  run leader(0, v1tov2); run vehicle(1, v1tov2, v3tov2); run tail(2, v3tov2);
+  run attacker(v1tov2, v3tov2)
+}  
+
+/* Original property: [](big_speed_difference => X ~ big_speed_difference)
+   Never: <>(big_speed_difference & X big_speed_difference)
+   */
+never              /* <>(big_speed_difference & X big_speed_difference) */
+      {
+          T0:
+                if
+                :: (vspeed > (lspeed+5)) -> goto Bigdiff
+		:: (vspeed < (lspeed-5)) -> goto Bigdiff
+		:: (vspeed > (tspeed+5)) -> goto Bigdiff
+		:: (vspeed < (tspeed-5)) -> goto Bigdiff
+		::  ((vspeed <= (lspeed+5)) && (vspeed >= (lspeed-5)) && (vspeed <= (lspeed+5)) && (vspeed >= (lspeed-5))) -> goto T0
+		fi;
+	Bigdiff:
+                if
+                :: (vspeed > (lspeed+5)) -> goto accept
+		:: (vspeed < (lspeed-5)) -> goto accept
+		:: (vspeed > (tspeed+5)) -> goto accept
+		:: (vspeed < (tspeed-5)) -> goto accept
+		::  ((vspeed <= (lspeed+5)) && (vspeed >= (lspeed-5)) && (vspeed <= (lspeed+5)) && (vspeed >= (lspeed-5))) -> goto T0
+		fi;
+          accept:
+                skip
+       }
